first proofs

SSA/Projects/RISCV64/removeToIntToNat.lean
@@ -1,33 +1,40 @@
-import SSA.Core.MLIRSyntax.EDSL
-set_option maxHeartbeats 1000000000000000000
+/- we import these specific mathlib libraries to use Nat.cast_ofNat and neg_neg lemmas. -/
+import Mathlib.Order.Lattice
+import Mathlib.Data.Nat.Cast.Defs
 
 /-!
   ## Dialect semantics bit-vectorization
-This file contains the `RV64` instruction semantics in a form that does not contain BitVec.toInt and BitVec.toNat.
+This file contains the `RV64` instruction semantics in a form that does
+not contain BitVec.toInt and BitVec.toNat.
 ToInt/ToNat calls hinder proof automation by bv_decide.
-To guarantee faithful rewrites of the dialect semantics as defined in Sail-Lean, this file also contains
-a proof for each rewrite.
-The instruction semantics suffixed by "bv" indicates that it is a transformed defintion where we removed
+To guarantee faithfullness to the semantics defined by the Sail-Lean RiscV64 model,
+we provide a proof with each rewrite that shows, that the toInt/ toNat free
+version is semantically equivalent to the defintion extracted from
+the Sail RiscV 64 modell in Lean. [1]
+
+[1]:
+
+The instruction semantics suffixed by "bv" indicates that it is
+the purely bit vector defintion where we removed
 toInt/toNat calls.
 -/
 
-/-  ## Additional introducded lemmas on bit vectors -/
-namespace pure_semantics
+/-! ## Helper Bit Vector Lemmas  -/
+/- The lemmas bellow are helper lemmas used within proofs throughout the file -/
+
 theorem sshiftRight_eq_sshiftRight_extractLsb {w : Nat}
     {lw : Nat} (hll : 2^lw = w) (hlw : lw > 0 )
-    (x y : BitVec w)(h : BitVec.toNat y < 2^lw ) : x.sshiftRight y.toNat = x.sshiftRight (y.extractLsb (lw - 1) 0).toNat := by
-    apply BitVec.eq_of_toNat_eq
-    simp
-    suffices y.toNat = (y.toNat % 2 ^ (lw - 1 + 1)) by
-      rw [← this ]
-    have : (lw - 1 + 1) = lw := by omega
-    rw [this, hll]
-    rw [Nat.mod_eq_of_lt]
-    rw [hll] at h
-    exact h
-
-theorem eq_of_toNat_eq3 {n} : ∀ {x y : BitVec n}, x.toNat = y.toNat → x = y
-  | ⟨_, _⟩, ⟨_, _⟩, rfl => rfl
+    (x y : BitVec w)(h : BitVec.toNat y < 2^lw ) :
+        x.sshiftRight y.toNat = x.sshiftRight (y.extractLsb (lw - 1) 0).toNat := by
+  apply BitVec.eq_of_toNat_eq
+  simp
+  suffices y.toNat = (y.toNat % 2 ^ (lw - 1 + 1)) by
+    rw [← this ]
+  have : (lw - 1 + 1) = lw := by omega
+  rw [this, hll]
+  rw [Nat.mod_eq_of_lt]
+  rw [hll] at h
+  exact h
 
 theorem sshiftRight_eq_setWidth_extractLsb_signExtend {w : Nat} (n : Nat) (x : BitVec w) :
     x.sshiftRight n =
@@ -38,11 +45,13 @@ theorem sshiftRight_eq_setWidth_extractLsb_signExtend {w : Nat} (n : Nat) (x : B
   simp [BitVec.getLsbD_signExtend]
   by_cases hni : (n + i) < w <;> simp [hni] <;> omega
 
-theorem BitVec.ofInt_toInt_eq_signExtend {w w' : Nat} {x : BitVec w} : BitVec.ofInt w' x.toInt = x.signExtend w' := by
+theorem BitVec.ofInt_toInt_eq_signExtend {w w' : Nat} {x : BitVec w} : BitVec.ofInt w' x.toInt
+      = x.signExtend w' := by
   apply BitVec.eq_of_toInt_eq
   by_cases hw' : w' ≤ w
-  · simp; rw [BitVec.toInt_signExtend_eq_toInt_bmod_of_le _ hw']
-  · simp at hw'
+  · simp
+    rw [BitVec.toInt_signExtend_eq_toInt_bmod_of_le _ hw']
+  · simp only [not_le] at hw'
     rw [BitVec.toInt_ofInt]
     rw [BitVec.toInt_signExtend_of_le (by omega)]
     have hxlt := @BitVec.two_mul_toInt_lt w x
@@ -53,7 +62,7 @@ theorem BitVec.ofInt_toInt_eq_signExtend {w w' : Nat} {x : BitVec w} : BitVec.of
       norm_cast
     rw [Int.bmod_eq_of_le_mul_two] <;> push_cast <;> omega
 
-theorem toInt_toInt_ofInt_eq_toNat_toNat_ofNa{w w' : Nat }{x y : BitVec w } (h : w' ≤ w):
+theorem toInt_toInt_ofInt_eq_toNat_toNat_ofNa {w w' : Nat }{x y : BitVec w } (h : w' ≤ w):
     BitVec.ofNat w' (x.toNat * y.toNat) = BitVec.ofInt w' (x.toInt * y.toInt) := by
   rw [BitVec.ofNat_mul]
   simp
@@ -63,12 +72,8 @@ theorem toInt_toInt_ofInt_eq_toNat_toNat_ofNa{w w' : Nat }{x y : BitVec w } (h :
   rw [BitVec.signExtend_eq_setWidth_of_le _ (by omega)]
   rw [BitVec.signExtend_eq_setWidth_of_le _ (by omega)]
 
-theorem neg_ofNat_eq_ofInt_neg {w : Nat} (x : Nat) :
-    - BitVec.ofNat w x = BitVec.ofInt w (- x) := by
-  apply BitVec.eq_of_toInt_eq
-  simp [BitVec.toInt_neg, BitVec.toInt_ofNat]
 
-@[simp]
+@[simp] -- we tag the lemma as a simp lemma
 theorem extractLsb'_eq_setWidth {x : BitVec w} : x.extractLsb' 0 n = x.setWidth n := by
   ext i hi
   simp?
@@ -92,36 +97,55 @@ theorem BitVec.setWidth_signExtend_eq_self {w w' : Nat} {x : BitVec w} (h : w �
   simp  [hi, BitVec.getLsbD_signExtend]
   omega
 
+theorem extractLsb_setWidth_of_lt (x : BitVec w) (hi lo v : Nat) (hilo : lo < hi) (hhi : hi < v):
+    BitVec.extractLsb hi lo (BitVec.setWidth v x) = BitVec.extractLsb hi lo x := by
+  simp only [BitVec.extractLsb]
+  ext k
+  simp only [BitVec.getElem_extractLsb', BitVec.getLsbD_setWidth, Bool.and_eq_right_iff_imp,
+    decide_eq_true_eq]
+  omega
+
+/- Proof in process. The following lemma does not yet exist in Lean's bit vector library.
+We are confident that this holds and the lemma is in process of being proven and
+added to the Lean's bit vector library.
+-/
+theorem toInt_smod {x y : BitVec w} :
+    (x.smod y).toInt = x.toInt.fmod y.toInt := by sorry
+
+
+/-! # ToNat and toInt-free RiscV instruction semantics -/
+
+namespace pure_semantics
 
 def ADDIW_pure64 (imm : BitVec 12) (rs1_val : BitVec 64) : BitVec 64 :=
-     BitVec.signExtend 64 (BitVec.setWidth 32 (BitVec.add (BitVec.signExtend 64 imm) rs1_val))
+    BitVec.signExtend 64 (BitVec.setWidth 32 (BitVec.add (BitVec.signExtend 64 imm) rs1_val))
 
 def UTYPE_pure64_lui (imm : BitVec 20) (pc : BitVec 64) : BitVec 64 :=
-  BitVec.signExtend 64 (imm ++ (0x000 : (BitVec 12)))
+    BitVec.signExtend 64 (imm ++ (0x000 : BitVec 12))
 
 def UTYPE_pure64_AUIPC (imm : BitVec 20) (pc : BitVec 64) : BitVec 64 :=
-  BitVec.add (BitVec.signExtend 64 (BitVec.append imm (0x000 : (BitVec 12)))) pc
+    BitVec.add (BitVec.signExtend 64 (BitVec.append imm (0x000 : BitVec 12))) pc
 
 def SHIFTIWOP_pure64_RISCV_SLLIW (shamt : BitVec 5) (rs1_val : BitVec 64) : BitVec 64 :=
-  BitVec.signExtend 64 (BitVec.shiftLeft (BitVec.extractLsb' 0 32 rs1_val) (shamt).toNat)
+    BitVec.signExtend 64 (BitVec.shiftLeft (BitVec.extractLsb' 0 32 rs1_val) (shamt).toNat)
 
 def SHIFTIWOP_pure64_RISCV_SLLIW_bv (shamt : BitVec 5) (rs1_val : BitVec 64) : BitVec 64 :=
-  BitVec.signExtend 64 ( (BitVec.extractLsb' 0 32 rs1_val)  <<< (shamt))
+    BitVec.signExtend 64 ((BitVec.extractLsb' 0 32 rs1_val)  <<< shamt)
 
 theorem SHIFTIWOP_pure64_RISCV_SLLIW_eq_SHIFTIWOP_pure64_RISCV_SLLIW_bv (shamt : BitVec 5) (rs1_val : BitVec 64) :
-  SHIFTIWOP_pure64_RISCV_SLLIW (shamt ) (rs1_val ) = SHIFTIWOP_pure64_RISCV_SLLIW_bv (shamt) (rs1_val) :=
+    SHIFTIWOP_pure64_RISCV_SLLIW (shamt ) (rs1_val) = SHIFTIWOP_pure64_RISCV_SLLIW_bv (shamt) (rs1_val) :=
   by
   unfold SHIFTIWOP_pure64_RISCV_SLLIW SHIFTIWOP_pure64_RISCV_SLLIW_bv
   rfl
 
 def SHIFTIWOP_pure64_RISCV_SRLIW (shamt : BitVec 5) (rs1_val : BitVec 64) : BitVec 64 :=
-  BitVec.signExtend 64 (BitVec.ushiftRight (BitVec.extractLsb' 0 32 rs1_val) (shamt).toNat)
+    BitVec.signExtend 64 (BitVec.ushiftRight (BitVec.extractLsb' 0 32 rs1_val) (shamt).toNat)
 
 def SHIFTIWOP_pure64_RISCV_SRLIW_bv (shamt : BitVec 5) (rs1_val : BitVec 64) : BitVec 64 :=
-  BitVec.signExtend 64 ( (BitVec.extractLsb' 0 32 rs1_val) >>> (shamt))
+    BitVec.signExtend 64 ((BitVec.extractLsb' 0 32 rs1_val) >>> (shamt))
 
 theorem  SHIFTIWOP_pure64_RISCV_SRLIW_eq_SHIFTIWOP_pure64_RISCV_SRLIW_bv (shamt : BitVec 5) (rs1_val : BitVec 64) :
-  SHIFTIWOP_pure64_RISCV_SRLIW (shamt) (rs1_val) =  SHIFTIWOP_pure64_RISCV_SRLIW_bv (shamt) (rs1_val) :=
+    SHIFTIWOP_pure64_RISCV_SRLIW (shamt) (rs1_val) =  SHIFTIWOP_pure64_RISCV_SRLIW_bv (shamt) (rs1_val) :=
   by
   unfold SHIFTIWOP_pure64_RISCV_SRLIW SHIFTIWOP_pure64_RISCV_SRLIW_bv
   rfl
@@ -132,103 +156,106 @@ def SHIFTIWOP_pure64_RISCV_SRAIW (shamt : BitVec 5) (rs1_val : BitVec 64) : BitV
        (BitVec.extractLsb
          (31 + shamt.toNat)
           shamt.toNat
-          (BitVec.signExtend ((32) + shamt.toNat) (BitVec.extractLsb 31 0 rs1_val))))
+          (BitVec.signExtend (32 + shamt.toNat) (BitVec.extractLsb 31 0 rs1_val))))
 
 def SHIFTIWOP_pure64_RISCV_SRAIW_bv (shamt : BitVec 5) (rs1_val : BitVec 64) : BitVec 64 :=
-  BitVec.signExtend 64 (BitVec.sshiftRight' (BitVec.extractLsb 31 0 rs1_val) shamt)
+    BitVec.signExtend 64 (BitVec.sshiftRight' (BitVec.extractLsb 31 0 rs1_val) shamt)
 
 theorem SHIFTIWOP_pure64_RISCV_SRAIW_eq_SHIFTIWOP_pure64_RISCV_SRAIW_bv (shamt : BitVec 5) (rs1_val : BitVec 64) :
-  SHIFTIWOP_pure64_RISCV_SRAIW (shamt) (rs1_val) = SHIFTIWOP_pure64_RISCV_SRAIW_bv (shamt) (rs1_val) :=
+    SHIFTIWOP_pure64_RISCV_SRAIW (shamt) (rs1_val) = SHIFTIWOP_pure64_RISCV_SRAIW_bv (shamt) (rs1_val) :=
   by
   unfold SHIFTIWOP_pure64_RISCV_SRAIW SHIFTIWOP_pure64_RISCV_SRAIW_bv
   rw [← sshiftRight_eq_setWidth_extractLsb_signExtend]
   rfl
 
 def SHIFTIOP_pure64_RISCV_SLLI (shamt : BitVec 6) (rs1_val : BitVec 64) : BitVec 64 :=
-  BitVec.shiftLeft rs1_val shamt.toNat
+    BitVec.shiftLeft rs1_val shamt.toNat
 
 def  SHIFTIOP_pure64_RISCV_SLLI_bv (shamt : BitVec 6) (rs1_val : BitVec 64) : BitVec 64 :=
-  rs1_val <<< shamt
+    rs1_val <<< shamt
 
 theorem SHIFTIOP_pure64_RISCV_SLLI_eq_SHIFTIOP_pure64_RISCV_SLLI_bv :
-  SHIFTIOP_pure64_RISCV_SLLI (shamt) (rs1_val) = SHIFTIOP_pure64_RISCV_SLLI_bv (shamt) (rs1_val) := by
+    SHIFTIOP_pure64_RISCV_SLLI (shamt) (rs1_val) = SHIFTIOP_pure64_RISCV_SLLI_bv (shamt) (rs1_val) := by
   unfold SHIFTIOP_pure64_RISCV_SLLI SHIFTIOP_pure64_RISCV_SLLI_bv
-  simp
+  simp only [BitVec.shiftLeft_eq, BitVec.shiftLeft_eq']
 
 def SHIFTIOP_pure64_RISCV_SRLI (shamt : BitVec 6) (rs1_val : BitVec 64) : BitVec 64 :=
-  BitVec.ushiftRight rs1_val shamt.toNat
+    BitVec.ushiftRight rs1_val shamt.toNat
 
 def SHIFTIOP_pure64_RISCV_SRLI_bv (shamt : BitVec 6) (rs1_val : BitVec 64) : BitVec 64 :=
-  rs1_val >>> shamt
+    rs1_val >>> shamt
 
 theorem SHIFTIOP_pure64_RISCV_SRLI_eq_SHIFTIOP_pure64_RISCV_SRLI_bv (shamt : BitVec 6) (rs1_val : BitVec 64) :
-  SHIFTIOP_pure64_RISCV_SRLI (shamt) (rs1_val) = SHIFTIOP_pure64_RISCV_SRLI_bv (shamt) (rs1_val) := by
+    SHIFTIOP_pure64_RISCV_SRLI (shamt) (rs1_val) = SHIFTIOP_pure64_RISCV_SRLI_bv (shamt) (rs1_val) := by
   unfold SHIFTIOP_pure64_RISCV_SRLI SHIFTIOP_pure64_RISCV_SRLI_bv
   simp
 
 def SHIFTIOP_pure64_RISCV_SRAI (shamt : BitVec 6) (rs1_val : BitVec 64): BitVec 64 :=
-  let value := rs1_val ;
-  let shift := shamt.toNat;
-  BitVec.setWidth 64 (BitVec.extractLsb (63 + shift) shift (BitVec.signExtend (64 + shift) value))
+    let value := rs1_val ;
+    let shift := shamt.toNat;
+    BitVec.setWidth 64 (BitVec.extractLsb (63 + shift) shift (BitVec.signExtend (64 + shift) value))
 
 def SHIFTIOP_pure64_RISCV_SRAI_bv (shamt : BitVec 6) (rs1_val : BitVec 64): BitVec 64 :=
-  BitVec.sshiftRight' rs1_val  shamt
+    BitVec.sshiftRight' rs1_val  shamt
 
 theorem SHIFTIOP_pure64_RISCV_SRAI_eq_SHIFTIOP_pure64_RISCV_SRAI_bv (shamt : BitVec 6) (rs1_val : BitVec 64) :
-  SHIFTIOP_pure64_RISCV_SRAI (shamt) (rs1_val ) = SHIFTIOP_pure64_RISCV_SRAI_bv (shamt) (rs1_val ) :=
+    SHIFTIOP_pure64_RISCV_SRAI (shamt) (rs1_val ) = SHIFTIOP_pure64_RISCV_SRAI_bv (shamt) (rs1_val ) :=
   by
   unfold SHIFTIOP_pure64_RISCV_SRAI SHIFTIOP_pure64_RISCV_SRAI_bv
-  simp
+  simp only [BitVec.sshiftRight_eq']
   rw [sshiftRight_eq_setWidth_extractLsb_signExtend]
 
 def RTYPEW_pure64_RISCV_ADDW (rs2_val : BitVec 64) (rs1_val : BitVec 64) : BitVec 64 :=
-  let rs1_val32 := BitVec.extractLsb' 0 32 rs1_val;
-  let rs2_val32 := BitVec.extractLsb' 0 32 rs2_val;
-  BitVec.signExtend 64 (BitVec.add rs1_val32 rs2_val32)
+    let rs1_val32 := BitVec.extractLsb' 0 32 rs1_val;
+    let rs2_val32 := BitVec.extractLsb' 0 32 rs2_val;
+    BitVec.signExtend 64 (BitVec.add rs1_val32 rs2_val32)
 
 def RTYPEW_pure64_RISCV_SUBW (rs2_val : BitVec 64) (rs1_val : BitVec 64) : BitVec 64 :=
-  let rs1_val32 := BitVec.extractLsb' 0 32 rs1_val;
-  let rs2_val32 := BitVec.extractLsb' 0 32 rs2_val;
-  BitVec.signExtend 64 (BitVec.sub rs1_val32 rs2_val32)
+    let rs1_val32 := BitVec.extractLsb' 0 32 rs1_val;
+    let rs2_val32 := BitVec.extractLsb' 0 32 rs2_val;
+    BitVec.signExtend 64 (BitVec.sub rs1_val32 rs2_val32)
 
 def RTYPEW_pure64_RISCV_SLLW (rs2_val : BitVec 64) (rs1_val : BitVec 64) : BitVec 64 :=
-  let rs1_val32 := BitVec.extractLsb' 0 32 rs1_val;
-  let rs2_val32 := BitVec.extractLsb' 0 32 rs2_val;
-  let shamt := BitVec.extractLsb' 0 5 rs2_val32;
-  BitVec.signExtend 64 (BitVec.shiftLeft rs1_val32 shamt.toNat)
+    let rs1_val32 := BitVec.extractLsb' 0 32 rs1_val;
+    let rs2_val32 := BitVec.extractLsb' 0 32 rs2_val;
+    let shamt := BitVec.extractLsb' 0 5 rs2_val32;
+    BitVec.signExtend 64 (BitVec.shiftLeft rs1_val32 shamt.toNat)
 
 def RTYPEW_pure64_RISCV_SLLW_bv (rs2_val : BitVec 64) (rs1_val : BitVec 64) : BitVec 64 :=
-  let rs1_val32 := BitVec.extractLsb' 0 32 rs1_val;
-  let rs2_val32 := BitVec.extractLsb' 0 32 rs2_val;
-  let shamt := BitVec.extractLsb' 0 5 rs2_val32;
-  BitVec.signExtend 64 (rs1_val32 <<< shamt)
+    let rs1_val32 := BitVec.extractLsb' 0 32 rs1_val;
+    let rs2_val32 := BitVec.extractLsb' 0 32 rs2_val;
+    let shamt := BitVec.extractLsb' 0 5 rs2_val32;
+    BitVec.signExtend 64 (rs1_val32 <<< shamt)
 
 theorem  RTYPEW_pure64_RISCV_SLLW_eq_RTYPEW_pure64_RISCV_SLLW_bv (rs2_val : BitVec 64) (rs1_val : BitVec 64) :
-  RTYPEW_pure64_RISCV_SLLW (rs2_val) (rs1_val) =  RTYPEW_pure64_RISCV_SLLW_bv (rs2_val) (rs1_val) :=
+    RTYPEW_pure64_RISCV_SLLW (rs2_val) (rs1_val) =  RTYPEW_pure64_RISCV_SLLW_bv (rs2_val) (rs1_val) :=
   by
   unfold RTYPEW_pure64_RISCV_SLLW RTYPEW_pure64_RISCV_SLLW_bv
   simp only [extractLsb'_eq_setWidth, Nat.reduceLeDiff, BitVec.setWidth_setWidth_of_le,
     BitVec.toNat_setWidth, Nat.reducePow, BitVec.shiftLeft_eq, BitVec.shiftLeft_eq']
 
 def RTYPEW_pure64_RISCV_SRLW (rs2_val : BitVec 64) (rs1_val : BitVec 64) : BitVec 64 :=
-  let rs1_val32 := BitVec.extractLsb' 0 32 rs1_val;
-  let rs2_val32 := BitVec.extractLsb' 0 32 rs2_val;
-  let shamt := BitVec.extractLsb' 0 5 rs2_val32;
-  BitVec.signExtend 64 (BitVec.ushiftRight rs1_val32 shamt.toNat)
+    let rs1_val32 := BitVec.extractLsb' 0 32 rs1_val;
+    let rs2_val32 := BitVec.extractLsb' 0 32 rs2_val;
+    let shamt := BitVec.extractLsb' 0 5 rs2_val32;
+    BitVec.signExtend 64 (BitVec.ushiftRight rs1_val32 shamt.toNat)
 
 def RTYPEW_pure64_RISCV_SRLW_bv (rs2_val : BitVec 64) (rs1_val : BitVec 64) : BitVec 64 :=
-  let rs1_val32 := BitVec.extractLsb' 0 32 rs1_val;
-  let rs2_val32 := BitVec.extractLsb' 0 32 rs2_val;
-  let shamt := BitVec.extractLsb' 0 5 rs2_val32;
-  BitVec.signExtend 64 (rs1_val32 >>> shamt)
+    let rs1_val32 := BitVec.extractLsb' 0 32 rs1_val;
+    let rs2_val32 := BitVec.extractLsb' 0 32 rs2_val;
+    let shamt := BitVec.extractLsb' 0 5 rs2_val32;
+    BitVec.signExtend 64 (rs1_val32 >>> shamt)
 
-theorem RTYPEW_pure64_RISCV_SLLW_eq_RTYPEW_pure64_RISCV_SRLW_bv (rs2_val : BitVec 64) (rs1_val : BitVec 64) :
-  RTYPEW_pure64_RISCV_SRLW (rs2_val) (rs1_val) =  RTYPEW_pure64_RISCV_SRLW_bv (rs2_val) (rs1_val) := by
+theorem RTYPEW_pure64_RISCV_SLLW_eq_RTYPEW_pure64_RISCV_SRLW_bv
+    (rs2_val : BitVec 64) (rs1_val : BitVec 64) :
+    RTYPEW_pure64_RISCV_SRLW (rs2_val) (rs1_val)
+    = RTYPEW_pure64_RISCV_SRLW_bv (rs2_val) (rs1_val) := by
   unfold RTYPEW_pure64_RISCV_SRLW RTYPEW_pure64_RISCV_SRLW_bv
-  simp
+  simp only [extractLsb'_eq_setWidth, Nat.reduceLeDiff, BitVec.setWidth_setWidth_of_le,
+    BitVec.toNat_setWidth, Nat.reducePow, BitVec.ushiftRight_eq, BitVec.ushiftRight_eq']
 
 def RTYPEW_pure64_RISCV_SRAW (rs2_val : BitVec 64) (rs1_val : BitVec 64) :=
-  BitVec.signExtend 64
+    BitVec.signExtend 64
            (BitVec.setWidth 32
               (BitVec.extractLsb
                  (31 + rs2_val.toNat % 4294967296 % 32)
@@ -237,46 +264,48 @@ def RTYPEW_pure64_RISCV_SRAW (rs2_val : BitVec 64) (rs1_val : BitVec 64) :=
                               (BitVec.extractLsb 31 0 rs1_val))))
 
 def RTYPEW_pure64_RISCV_SRAW_bv (rs2_val : BitVec 64) (rs1_val : BitVec 64) :=
-  BitVec.signExtend 64
-  (BitVec.sshiftRight' (BitVec.extractLsb 31 0 rs1_val)  (BitVec.extractLsb 4 0 rs2_val))
+    BitVec.signExtend 64
+    (BitVec.sshiftRight' (BitVec.extractLsb 31 0 rs1_val) (BitVec.extractLsb 4 0 rs2_val))
 
-theorem RTYPEW_pure64_RISCV_SRAW_eq_RTYPEW_pure64_RISCV_SRAW_bv (rs2_val : BitVec 64) (rs1_val : BitVec 64) :
-  RTYPEW_pure64_RISCV_SRAW (rs2_val) (rs1_val) = RTYPEW_pure64_RISCV_SRAW_bv (rs2_val) (rs1_val) :=
+theorem RTYPEW_pure64_RISCV_SRAW_eq_RTYPEW_pure64_RISCV_SRAW_bv
+    (rs2_val : BitVec 64) (rs1_val : BitVec 64) :
+    RTYPEW_pure64_RISCV_SRAW (rs2_val) (rs1_val)
+    = RTYPEW_pure64_RISCV_SRAW_bv (rs2_val) (rs1_val) :=
   by
   unfold RTYPEW_pure64_RISCV_SRAW RTYPEW_pure64_RISCV_SRAW_bv
   rw [← sshiftRight_eq_setWidth_extractLsb_signExtend]
   simp
 
 def RTYPE_pure64_RISCV_ADD (rs2_val : BitVec 64) (rs1_val : BitVec 64) : BitVec 64 :=
-  BitVec.add rs1_val rs2_val
+    BitVec.add rs1_val rs2_val
 
 def RTYPE_pure64_RISCV_SLT (rs2_val : BitVec 64) (rs1_val : BitVec 64) : BitVec 64 :=
-  let b := BitVec.slt rs1_val rs2_val;
-  BitVec.setWidth 64 (BitVec.ofBool b)
+    let b := BitVec.slt rs1_val rs2_val;
+    BitVec.setWidth 64 (BitVec.ofBool b)
 
 def RTYPE_pure64_RISCV_SLTU (rs2_val : BitVec 64) (rs1_val : BitVec 64) : BitVec 64 :=
-  let b := BitVec.ult rs1_val rs2_val;
-  BitVec.setWidth 64 (BitVec.ofBool b)
+    let b := BitVec.ult rs1_val rs2_val;
+    BitVec.setWidth 64 (BitVec.ofBool b)
 
 def RTYPE_pure64_RISCV_AND (rs2_val : BitVec 64) (rs1_val : BitVec 64) : BitVec 64 :=
-  BitVec.and rs2_val rs1_val
+    BitVec.and rs2_val rs1_val
 
 def RTYPE_pure64_RISCV_OR(rs2_val : BitVec 64) (rs1_val : BitVec 64) : BitVec 64 :=
-  BitVec.or rs2_val rs1_val
+    BitVec.or rs2_val rs1_val
 
 def RTYPE_pure64_RISCV_XOR(rs2_val : BitVec 64) (rs1_val : BitVec 64) : BitVec 64 :=
-  BitVec.xor rs2_val rs1_val
+    BitVec.xor rs2_val rs1_val
 
 def RTYPE_pure64_RISCV_SLL (rs2_val : BitVec 64) (rs1_val : BitVec 64) : BitVec 64 :=
-  let shamt := (BitVec.extractLsb 5 0 rs2_val).toNat;
-  BitVec.shiftLeft rs1_val shamt
+    let shamt := (BitVec.extractLsb 5 0 rs2_val).toNat;
+    BitVec.shiftLeft rs1_val shamt
 
 def RTYPE_pure64_RISCV_SLL_bv (rs2_val : BitVec 64) (rs1_val : BitVec 64) : BitVec 64 :=
-  let shamt := (BitVec.extractLsb 5 0 rs2_val);
-  rs1_val <<< shamt
+    let shamt := (BitVec.extractLsb 5 0 rs2_val);
+    rs1_val <<< shamt
 
-theorem RTYPE_pure64_RISCV_SLL_eq_RTYPE_pure64_RISCV_SLL_bv  (rs2_val : BitVec 64) (rs1_val : BitVec 64) :
-  RTYPE_pure64_RISCV_SLL (rs2_val) (rs1_val)= RTYPE_pure64_RISCV_SLL_bv (rs2_val) (rs1_val) := by
+theorem RTYPE_pure64_RISCV_SLL_eq_RTYPE_pure64_RISCV_SLL_bv (rs2_val : BitVec 64) (rs1_val : BitVec 64) :
+    RTYPE_pure64_RISCV_SLL (rs2_val) (rs1_val)= RTYPE_pure64_RISCV_SLL_bv (rs2_val) (rs1_val) := by
   unfold RTYPE_pure64_RISCV_SLL  RTYPE_pure64_RISCV_SLL_bv
   simp
 
@@ -289,7 +318,7 @@ def RTYPE_pure64_RISCV_SRL_bv (rs2_val : BitVec 64) (rs1_val : BitVec 64) : BitV
   rs1_val >>> shamt
 
 theorem RTYPE_pure64_RISCV_SRL_eq_RTYPE_pure64_RISCV_SRL_bv  (rs2_val : BitVec 64) (rs1_val : BitVec 64) :
-  RTYPE_pure64_RISCV_SRL (rs2_val) (rs1_val) = RTYPE_pure64_RISCV_SRL_bv (rs2_val) (rs1_val) :=
+    RTYPE_pure64_RISCV_SRL (rs2_val) (rs1_val) = RTYPE_pure64_RISCV_SRL_bv (rs2_val) (rs1_val) :=
   by
   unfold RTYPE_pure64_RISCV_SRL RTYPE_pure64_RISCV_SRL_bv
   simp
@@ -298,7 +327,7 @@ def RTYPE_pure64_RISCV_SUB (rs2_val : BitVec 64) (rs1_val : BitVec 64) : BitVec 
   BitVec.sub rs1_val rs2_val
 
 def RTYPE_pure64_RISCV_SRA (rs2_val : BitVec 64) (rs1_val : BitVec 64) :=
-  BitVec.setWidth 64
+    BitVec.setWidth 64
       (BitVec.extractLsb
         (63 + (BitVec.extractLsb 5 0 rs2_val).toNat)
         (BitVec.extractLsb 5 0 rs2_val).toNat
@@ -306,27 +335,28 @@ def RTYPE_pure64_RISCV_SRA (rs2_val : BitVec 64) (rs1_val : BitVec 64) :=
           (64 + (BitVec.extractLsb 5 0 rs2_val).toNat) rs1_val))
 
 def RTYPE_pure64_RISCV_SRA_bv (rs2_val : BitVec 64) (rs1_val : BitVec 64) : BitVec 64 :=
-  BitVec.sshiftRight' rs1_val (BitVec.extractLsb 5 0 rs2_val)
+    BitVec.sshiftRight' rs1_val (BitVec.extractLsb 5 0 rs2_val)
 
 theorem RTYPE_pure64_RISCV_SRA_eqRTYPE_pure64_RISCV_SRA_bv (rs2_val : BitVec 64) (rs1_val : BitVec 64) :
-  RTYPE_pure64_RISCV_SRA  (rs2_val) (rs1_val) = RTYPE_pure64_RISCV_SRA_bv (rs2_val) (rs1_val) := by
+    RTYPE_pure64_RISCV_SRA  (rs2_val) (rs1_val) = RTYPE_pure64_RISCV_SRA_bv (rs2_val) (rs1_val) := by
   unfold RTYPE_pure64_RISCV_SRA RTYPE_pure64_RISCV_SRA_bv
   rw [BitVec.sshiftRight']
   rw [sshiftRight_eq_setWidth_extractLsb_signExtend]
 
 def REMW_pure64_unsigned (rs2_val : BitVec 64) (rs1_val : BitVec 64): BitVec 64 :=
- BitVec.signExtend 64
-    (BitVec.extractLsb' 0 32
-      (BitVec.ofInt 33
-        (if ((BitVec.extractLsb 31 0 rs2_val).toNat : Int) = 0 then ↑(BitVec.extractLsb 31 0 rs1_val).toNat
-        else ((BitVec.extractLsb 31 0 rs1_val).toNat : Int).tmod ↑(BitVec.extractLsb 31 0 rs2_val).toNat)))
+    BitVec.signExtend 64
+      (BitVec.extractLsb' 0 32
+        (BitVec.ofInt 33
+          (if ((BitVec.extractLsb 31 0 rs2_val).toNat : Int) = 0 then ↑(BitVec.extractLsb 31 0 rs1_val).toNat
+          else ((BitVec.extractLsb 31 0 rs1_val).toNat : Int).tmod ↑(BitVec.extractLsb 31 0 rs2_val).toNat)))
 
-def REMW_pure64_unsigned_bv (rs2_val : (BitVec 64)) (rs1_val : (BitVec 64)) : BitVec 64 :=
-  BitVec.signExtend 64
+def REMW_pure64_unsigned_bv (rs2_val : BitVec 64) (rs1_val : BitVec 64) : BitVec 64 :=
+    BitVec.signExtend 64
       ((BitVec.extractLsb 31 0 rs1_val).umod (BitVec.extractLsb 31 0 rs2_val))
 
 theorem REMW_pure64_unsigned_eq_REMW_pure64_unsigned_bv (rs2_val : BitVec 64) (rs1_val : BitVec 64) :
-  REMW_pure64_unsigned (rs2_val : BitVec 64) (rs1_val : BitVec 64) =  REMW_pure64_unsigned_bv (rs2_val : (BitVec 64)) (rs1_val : (BitVec 64)) :=
+  REMW_pure64_unsigned (rs2_val : BitVec 64) (rs1_val : BitVec 64)
+      = REMW_pure64_unsigned_bv (rs2_val : BitVec 64) (rs1_val : BitVec 64) :=
   by
   unfold  REMW_pure64_unsigned REMW_pure64_unsigned_bv
   rw [extractLsb'_ofInt_eq_ofInt (h:= by simp)]
@@ -366,22 +396,22 @@ theorem REMW_pure64_unsigned_eq_REMW_pure64_unsigned_bv (rs2_val : BitVec 64) (r
         Nat.shiftRight_zero, Nat.sub_zero, Nat.reduceAdd, Int.natCast_emod, Nat.cast_ofNat]
       rfl
 
-def REMW_pure64_signed (rs2_val : (BitVec 64)) (rs1_val : (BitVec 64)) : BitVec 64 :=
+def REMW_pure64_signed (rs2_val : BitVec 64) (rs1_val : BitVec 64) : BitVec 64 :=
   BitVec.signExtend 64
     (BitVec.extractLsb' 0 32
       (BitVec.ofInt (33)
         (if (BitVec.extractLsb 31 0 rs2_val).toInt = 0 then (BitVec.extractLsb 31 0 rs1_val).toInt
         else (BitVec.extractLsb 31 0 rs1_val).toInt.tmod (BitVec.extractLsb 31 0 rs2_val).toInt)))
 
-def REMW_pure64_signed_bv (rs2_val : (BitVec 64)) (rs1_val : (BitVec 64)) : BitVec 64 :=
+def REMW_pure64_signed_bv (rs2_val : BitVec 64) (rs1_val : BitVec 64) : BitVec 64 :=
   BitVec.signExtend 64
       ((BitVec.extractLsb 31 0 rs1_val).srem (BitVec.extractLsb 31 0 rs2_val))
 
-theorem REMW_pure64_signed_eq_REMW_pure64_signed  (rs2_val : BitVec 64) (rs1_val : BitVec 64) :
+theorem REMW_pure64_signed_eq_REMW_pure64_signed (rs2_val : BitVec 64) (rs1_val : BitVec 64) :
    REMW_pure64_signed (rs2_val) (rs1_val) = REMW_pure64_signed_bv (rs2_val) (rs1_val) :=
     by
     unfold REMW_pure64_signed REMW_pure64_signed_bv
-    rw [extractLsb'_ofInt_eq_ofInt (h:= by simp )]
+    rw [extractLsb'_ofInt_eq_ofInt (h:= by simp)]
     congr
     split
     case e_x.isTrue ht  =>
@@ -396,18 +426,12 @@ theorem REMW_pure64_signed_eq_REMW_pure64_signed  (rs2_val : BitVec 64) (rs1_val
       rw [BitVec.ofInt_toInt]
 
 def REM_pure64_unsigned (rs2_val : BitVec 64) (rs1_val : BitVec 64) : BitVec 64  :=
-  BitVec.extractLsb' 0 64
-    (BitVec.ofInt (65) (if (rs2_val.toNat: Int) = 0 then (rs1_val.toNat: Int)  else ((rs1_val.toNat : Int )).tmod (rs2_val.toNat : Int)))
+    BitVec.extractLsb' 0 64
+    (BitVec.ofInt 65 (if (rs2_val.toNat: Int) = 0 then (rs1_val.toNat: Int)  else ((rs1_val.toNat : Int )).tmod (rs2_val.toNat : Int)))
 
 def REM_pure64_unsigned_bv (rs2_val : BitVec 64) (rs1_val : BitVec 64) : BitVec 64  :=
-   (if (rs2_val) = 0 then (rs1_val)  else ((rs1_val).umod (rs2_val)))
+    (if rs2_val = 0 then rs1_val  else ((rs1_val).umod (rs2_val)))
 
-/- proof in process. The following lemma does not yet exist in Lean's bit vector library.
-We are confident that this holds and the lemma is in process of being proven and
-added to the bit vector library.
--/
-theorem toInt_smod {x y : BitVec w} :
-    (x.smod y).toInt = x.toInt.fmod y.toInt := by sorry
 
 theorem  REM_pure64_unsigned_eq_REM_pure64_unsigned_bv (rs2_val : BitVec 64) (rs1_val : BitVec 64) :
     REM_pure64_unsigned (rs2_val) (rs1_val) = REM_pure64_unsigned_bv (rs2_val) (rs1_val) := by
@@ -433,13 +457,13 @@ theorem  REM_pure64_unsigned_eq_REM_pure64_unsigned_bv (rs2_val : BitVec 64) (rs
 
 def REM_pure64_signed (rs2_val : BitVec 64) (rs1_val : BitVec 64) : BitVec 64  :=
     BitVec.extractLsb' 0 64
-    (BitVec.ofInt (65) (if rs2_val.toInt = 0 then rs1_val.toInt else rs1_val.toInt.tmod rs2_val.toInt))
+    (BitVec.ofInt 65 (if rs2_val.toInt = 0 then rs1_val.toInt else rs1_val.toInt.tmod rs2_val.toInt))
 
 def REM_pure64_signed_bv (rs2_val : BitVec 64) (rs1_val : BitVec 64) : BitVec 64 :=
    rs1_val.srem rs2_val
 
 theorem REM_pure64_signed_eq_REM_pure64_signed_bv (rs2_val : BitVec 64) (rs1_val : BitVec 64) :
-    REM_pure64_signed (rs2_val) (rs1_val) = REM_pure64_signed_bv (rs2_val) (rs1_val) := by
+    REM_pure64_signed rs2_val rs1_val = REM_pure64_signed_bv rs2_val rs1_val := by
   unfold REM_pure64_signed REM_pure64_signed_bv
   rw [extractLsb'_ofInt_eq_ofInt (h:= by simp)]
   split
@@ -463,107 +487,92 @@ def MULW_pure64_bv (rs2_val : BitVec 64) (rs1_val : BitVec 64) : BitVec 64 :=
     (((BitVec.extractLsb 31 0 rs1_val) * (BitVec.extractLsb 31 0 rs2_val)))
 
 theorem MULW_pure64_eq_MULW_pure64_bv (rs2_val : BitVec 64) (rs1_val : BitVec 64)  :
-  MULW_pure64 (rs2_val) (rs1_val) = MULW_pure64_bv  (rs2_val) (rs1_val) :=
-    by
-    unfold MULW_pure64 MULW_pure64_bv
-    rw [extractLsb'_ofInt_eq_ofInt (h:= by simp)]
-    rw [BitVec.extractLsb]
-    simp only [Nat.sub_zero, Nat.reduceAdd]
-    rw [extractLsb'_ofInt_eq_ofInt (h:= by simp)]
-    congr
-    apply BitVec.eq_of_toInt_eq
-    simp only [BitVec.toInt_extractLsb, Nat.shiftRight_zero, Nat.sub_zero, Nat.reduceAdd,
-      Nat.reducePow, BitVec.toInt_ofInt, Int.mul_bmod_bmod, Int.bmod_mul_bmod, BitVec.toInt_mul]
+    MULW_pure64 rs2_val rs1_val = MULW_pure64_bv rs2_val rs1_val :=
+  by
+  unfold MULW_pure64 MULW_pure64_bv
+  rw [extractLsb'_ofInt_eq_ofInt (h:= by simp)]
+  rw [BitVec.extractLsb]
+  simp only [Nat.sub_zero, Nat.reduceAdd]
+  rw [extractLsb'_ofInt_eq_ofInt (h:= by simp)]
+  congr
+  apply BitVec.eq_of_toInt_eq
+  simp only [BitVec.toInt_extractLsb, Nat.shiftRight_zero, Nat.sub_zero, Nat.reduceAdd,
+    Nat.reducePow, BitVec.toInt_ofInt, Int.mul_bmod_bmod, Int.bmod_mul_bmod, BitVec.toInt_mul]
 
 def MUL_pure64_fff (rs2_val : BitVec 64) (rs1_val : BitVec 64) : BitVec 64 :=
      BitVec.extractLsb 63 0 (BitVec.extractLsb' 0 128 (BitVec.ofInt 129 (rs1_val.toNat * rs2_val.toNat)))
 
 def MUL_pure64_fff_bv (rs2_val : BitVec 64) (rs1_val : BitVec 64) : BitVec 64 :=  rs2_val * rs1_val
 
-theorem MUL_pure64_fff_eq_MUL_pure64_fff_bv (rs2_val : BitVec 64) (rs1_val : BitVec 64) :  MUL_pure64_fff  (rs2_val) (rs1_val)
-    = MUL_pure64_fff_bv  (rs2_val) (rs1_val ) := by
-    simp only  [MUL_pure64_fff,  MUL_pure64_fff_bv]
-    apply BitVec.eq_of_toNat_eq
-    simp only [HMul.hMul, Mul.mul]
-    simp only [Nat.sub_zero, Nat.reduceAdd, Int.mul_def, BitVec.extractLsb_toNat,
-      BitVec.extractLsb'_toNat, BitVec.toNat_ofInt, Nat.reducePow, Nat.cast_ofNat,
-      Nat.shiftRight_zero, Nat.reduceDvd, Nat.mod_mod_of_dvd, BitVec.mul_eq, BitVec.toNat_mul]
-    congr
-    norm_cast
-    rw [Int.toNat_natCast]
-    rw [Nat.mod_eq_of_lt]
-    ac_rfl
-    have aa := BitVec.isLt rs1_val
-    have bb := BitVec.isLt rs2_val
-    have := @Nat.mul_lt_mul'' _ _ _ _ aa bb
-    simp only [Nat.reducePow, Nat.reduceMul] at this
-    omega
+theorem MUL_pure64_fff_eq_MUL_pure64_fff_bv (rs2_val : BitVec 64) (rs1_val : BitVec 64) :
+    MUL_pure64_fff  rs2_val rs1_val = MUL_pure64_fff_bv rs2_val rs1_val := by
+  simp only  [MUL_pure64_fff,  MUL_pure64_fff_bv]
+  apply BitVec.eq_of_toNat_eq
+  simp only [HMul.hMul, Mul.mul]
+  simp only [Nat.sub_zero, Nat.reduceAdd, Int.mul_def, BitVec.extractLsb_toNat,
+    BitVec.extractLsb'_toNat, BitVec.toNat_ofInt, Nat.reducePow, Nat.cast_ofNat,
+    Nat.shiftRight_zero, Nat.reduceDvd, Nat.mod_mod_of_dvd, BitVec.mul_eq, BitVec.toNat_mul]
+  congr
+  norm_cast
+  rw [Int.toNat_natCast]
+  rw [Nat.mod_eq_of_lt]
+  ac_rfl
+  have aa := BitVec.isLt rs1_val
+  have bb := BitVec.isLt rs2_val
+  have := @Nat.mul_lt_mul'' _ _ _ _ aa bb
+  simp only [Nat.reducePow, Nat.reduceMul] at this
+  omega
 
 def  MUL_pure64_fft (rs2_val : BitVec 64) (rs1_val : BitVec 64) : BitVec 64 :=
-  BitVec.extractLsb 63 0
-    (BitVec.extractLsb' 0 128
-      (BitVec.ofInt 129 (Int.ofNat (Int.mul (Int.ofNat rs1_val.toNat)  (rs2_val.toInt)).toNat)))
-
--- no risc-v instruction maps to this multiplication with the combination of flags ftf.
-def MUL_pure64_ftf (rs2_val : BitVec 64) (rs1_val : BitVec 64)  : BitVec 64 :=
-  BitVec.extractLsb 63 0 (BitVec.extractLsb' 0 128 (BitVec.ofInt 129 (rs1_val.toInt * rs2_val.toNat)))
-
-def MUL_pure64_ftf_bv (rs2_val : BitVec 64) (rs1_val : BitVec 64) :=
-   BitVec.extractLsb 63 0 ( (rs1_val * rs2_val))
+    BitVec.extractLsb 63 0
+      (BitVec.extractLsb' 0 128
+        (BitVec.ofInt 129 (Int.ofNat (Int.mul (Int.ofNat rs1_val.toNat)  (rs2_val.toInt)).toNat)))
 
 def MUL_pure64_tff (rs2_val : BitVec 64) (rs1_val : BitVec 64) : BitVec 64 :=
-  BitVec.extractLsb 127 64 (BitVec.extractLsb' 0 128 (BitVec.ofInt 129 (rs1_val.toNat * rs2_val.toNat)))
+    BitVec.extractLsb 127 64 (BitVec.extractLsb' 0 128 (BitVec.ofInt 129 (rs1_val.toNat * rs2_val.toNat)))
 
 def MUL_pure64_tff_bv  (rs2_val : BitVec 64) (rs1_val : BitVec 64) : BitVec 64 :=
    BitVec.extractLsb 127 64 (BitVec.extractLsb' 0 128 ((BitVec.zeroExtend 128 rs1_val)  * (BitVec.zeroExtend 128 rs2_val)))
 
 theorem MUL_pure64_tff_eq_MUL_pure64_tff_bv  (rs2_val : BitVec 64) (rs1_val : BitVec 64)  :
-  MUL_pure64_tff (rs2_val) (rs1_val) = MUL_pure64_tff_bv (rs2_val) (rs1_val) := by
-    unfold  MUL_pure64_tff MUL_pure64_tff_bv
-    suffices (BitVec.extractLsb' 0 128 (BitVec.ofInt 129 (↑rs1_val.toNat * ↑rs2_val.toNat))) =
+    MUL_pure64_tff (rs2_val) (rs1_val) = MUL_pure64_tff_bv (rs2_val) (rs1_val) := by
+  unfold  MUL_pure64_tff MUL_pure64_tff_bv
+  suffices (BitVec.extractLsb' 0 128 (BitVec.ofInt 129 (↑rs1_val.toNat * ↑rs2_val.toNat))) =
                  (BitVec.extractLsb' 0 128 (BitVec.zeroExtend 128 rs1_val * BitVec.zeroExtend 128 rs2_val))
-      by
-      congr
-    apply BitVec.eq_of_toNat_eq
-    simp only [HMul.hMul, Mul.mul]
-    simp only [Int.mul_def, extractLsb'_eq_setWidth, BitVec.toNat_setWidth, BitVec.toNat_ofInt,
+    by
+    congr
+  apply BitVec.eq_of_toNat_eq
+  simp only [HMul.hMul, Mul.mul]
+  simp only [Int.mul_def, extractLsb'_eq_setWidth, BitVec.toNat_setWidth, BitVec.toNat_ofInt,
       Nat.reducePow, Nat.cast_ofNat, BitVec.truncate_eq_setWidth, BitVec.mul_eq,
       BitVec.extractLsb'_eq_self, BitVec.toNat_mul, Nat.mul_mod_mod, Nat.mod_mul_mod]
-    congr
-    norm_cast
-    rw [Int.toNat_natCast]
-    have aa := BitVec.isLt rs1_val
-    have bb := BitVec.isLt rs2_val
-    have cc : 680564733841876926926749214863536422912 = 2^129 := by native_decide
-    have aaa : rs1_val.toNat >= 0 := by simp
-    have bbb : rs2_val.toNat >= 0 := by simp
-    rw [Nat.mod_eq_of_lt (h:=
+  congr
+  norm_cast
+  rw [Int.toNat_natCast]
+  have aa := BitVec.isLt rs1_val
+  have bb := BitVec.isLt rs2_val
+  have cc : 680564733841876926926749214863536422912 = 2^129 := by native_decide
+  have aaa : rs1_val.toNat >= 0 := by simp
+  have bbb : rs2_val.toNat >= 0 := by simp
+  rw [Nat.mod_eq_of_lt (h:=
       by
       rw [cc]
-      have := Nat.mul_lt_mul'' (a := rs1_val.toNat) (b := rs2_val.toNat) (c := 2 ^ 64) (d := 2 ^ 64) aa bb
+      have := Nat.mul_lt_mul''
+        (a := rs1_val.toNat) (b := rs2_val.toNat) (c := 2 ^ 64) (d := 2 ^ 64) aa bb
       omega )]
-    have := @Nat.mul_lt_mul'' _ _ _ _ aa bb
-    simp only [Nat.reducePow, Nat.reduceMul] at this
-    omega
-
-theorem extractLsb_setWidth_of_lt (x : BitVec w) (hi lo v : Nat) (hilo : lo < hi) (hhi : hi < v):
-    BitVec.extractLsb hi lo (BitVec.setWidth v x) = BitVec.extractLsb hi lo x := by
-  simp only [BitVec.extractLsb]
-  ext k
-  simp only [BitVec.getElem_extractLsb', BitVec.getLsbD_setWidth, Bool.and_eq_right_iff_imp,
-    decide_eq_true_eq]
+  have := @Nat.mul_lt_mul'' _ _ _ _ aa bb
   omega
 
 def MUL_pure64_ttf (rs2_val : BitVec 64) (rs1_val : BitVec 64) : BitVec 64 :=
-  BitVec.extractLsb 127 64 (BitVec.extractLsb' 0 128 (BitVec.ofInt 129 (rs1_val.toInt * rs2_val.toNat)))
+    BitVec.extractLsb 127 64 (BitVec.extractLsb' 0 128 (BitVec.ofInt 129 (rs1_val.toInt * rs2_val.toNat)))
 
 def MUL_pure64_ttf_bv (rs2_val : BitVec 64) (rs1_val : BitVec 64) : BitVec 64 :=
-  BitVec.extractLsb 127 64 (((BitVec.signExtend 129 rs1_val ) * (BitVec.zeroExtend 129 rs2_val )))
+    BitVec.extractLsb 127 64 (((BitVec.signExtend 129 rs1_val ) * (BitVec.zeroExtend 129 rs2_val )))
 
 theorem MUL_pure64_ttf_eq_MUL_pure64_ttf_bv (rs2_val : BitVec 64) (rs1_val : BitVec 64) :
-   MUL_pure64_ttf (rs2_val) (rs1_val) = MUL_pure64_ttf_bv (rs2_val) (rs1_val) := by
+    MUL_pure64_ttf (rs2_val) (rs1_val) = MUL_pure64_ttf_bv (rs2_val) (rs1_val) := by
   unfold MUL_pure64_ttf MUL_pure64_ttf_bv
-  simp
+  simp only [extractLsb'_eq_setWidth, BitVec.truncate_eq_setWidth]
   have h1 : rs1_val.toInt = (rs1_val.signExtend 129).toInt := by
       simp only [Nat.reduceLeDiff, BitVec.toInt_signExtend_of_le]
   simp only [h1]
@@ -580,13 +589,13 @@ theorem MUL_pure64_ttf_eq_MUL_pure64_ttf_bv (rs2_val : BitVec 64) (rs1_val : Bit
   rw [extractLsb_setWidth_of_lt (hi := 127) (lo := 64) (v := 128) (x := BitVec.signExtend 129 rs1_val * BitVec.setWidth 129 rs2_val) (by omega) (by omega)]
 
 def MUL_pure64_ftt (rs2_val : BitVec 64) (rs1_val : BitVec 64) : BitVec 64 :=
-  BitVec.extractLsb 63 0 (BitVec.extractLsb' 0 128 (BitVec.ofInt 129 (rs1_val.toInt * rs2_val.toInt)))
+    BitVec.extractLsb 63 0 (BitVec.extractLsb' 0 128 (BitVec.ofInt 129 (rs1_val.toInt * rs2_val.toInt)))
 
 def MUL_pure64_ftt_bv  (rs2_val : BitVec 64) (rs1_val : BitVec 64) : BitVec 64 :=
-  rs2_val * rs1_val
+    rs2_val * rs1_val
 
-theorem MUL_pure64_ftt_eq_MUL_pure64_ftt_bv (rs2_val : BitVec 64) (rs1_val : BitVec 64) :  MUL_pure64_ftt  (rs2_val) (rs1_val )
-     = MUL_pure64_ftt_bv  (rs2_val) (rs1_val ) :=
+theorem MUL_pure64_ftt_eq_MUL_pure64_ftt_bv (rs2_val : BitVec 64) (rs1_val : BitVec 64) :
+    MUL_pure64_ftt  (rs2_val) (rs1_val) = MUL_pure64_ftt_bv (rs2_val) (rs1_val) :=
   by
   unfold  MUL_pure64_ftt  MUL_pure64_ftt_bv
   rw [BitVec.extractLsb]
@@ -605,13 +614,13 @@ theorem MUL_pure64_ftt_eq_MUL_pure64_ftt_bv (rs2_val : BitVec 64) (rs1_val : Bit
   ac_nf
 
 def MUL_pure64_ttt (rs2_val : BitVec 64) (rs1_val : BitVec 64) : BitVec 64 :=
-  BitVec.extractLsb 127 64 (BitVec.extractLsb' 0 128 (BitVec.ofInt 129 (rs1_val.toInt * rs2_val.toInt)))
+    BitVec.extractLsb 127 64 (BitVec.extractLsb' 0 128 (BitVec.ofInt 129 (rs1_val.toInt * rs2_val.toInt)))
 
 def MUL_pure64_ttt_bv  (rs2_val : BitVec 64) (rs1_val : BitVec 64) : BitVec 64 :=
- BitVec.extractLsb 127 64 ((BitVec.signExtend 129 rs1_val) *  (BitVec.signExtend 129 rs2_val))
+    BitVec.extractLsb 127 64 ((BitVec.signExtend 129 rs1_val) * (BitVec.signExtend 129 rs2_val))
 
 theorem MUL_pure64_ttt_eq_MUL_pure64_ttt_bv (rs2_val : BitVec 64) (rs1_val : BitVec 64) :
-   MUL_pure64_ttt rs2_val rs1_val  = MUL_pure64_ttt_bv rs2_val rs1_val :=
+    MUL_pure64_ttt rs2_val rs1_val = MUL_pure64_ttt_bv rs2_val rs1_val :=
    by
     unfold MUL_pure64_ttt_bv MUL_pure64_ttt
     have : rs1_val.toInt = (rs1_val.signExtend 129).toInt := by
@@ -624,333 +633,4 @@ theorem MUL_pure64_ttt_eq_MUL_pure64_ttt_bv (rs2_val : BitVec 64) (rs1_val : Bit
     simp only [BitVec.ofInt_toInt, extractLsb'_eq_setWidth]
     rw [extractLsb_setWidth_of_lt (hi := 127) (lo := 64) (v := 128) (x := BitVec.signExtend 129 rs1_val * BitVec.signExtend 129 rs2_val) (by omega)]
     simp
-
--- to do
-def DIVW_pure64_signed (rs2_val : BitVec 64) (rs1_val : BitVec 64) : BitVec 64 :=
-  BitVec.signExtend 64
-    (BitVec.extractLsb' 0 32
-      (BitVec.ofInt 33
-        (if
-            2147483647 <
-              if (BitVec.extractLsb 31 0 rs2_val).toInt = 0 then -1
-              else (BitVec.extractLsb 31 0 rs1_val).toInt.tdiv (BitVec.extractLsb 31 0 rs2_val).toInt then
-          -2147483648
-        else
-          if (BitVec.extractLsb 31 0 rs2_val).toInt = 0 then -1
-          else (BitVec.extractLsb 31 0 rs1_val).toInt.tdiv (BitVec.extractLsb 31 0 rs2_val).toInt)))
--- to do
-def  DIVW_pure64_unsigned (rs2_val : BitVec 64) (rs1_val : BitVec 64) : BitVec 64 :=
-       BitVec.signExtend 64
-    (BitVec.extractLsb' 0 32
-      (BitVec.ofInt 33
-        (if (rs2_val.toNat: Int)  % 4294967296 = 0 then -1
-        else ((rs1_val.toNat : Int) % 4294967296).tdiv ((rs2_val.toNat : Int) % 4294967296))))
-
-def DIV_pure64_signed (rs2_val : BitVec 64) (rs1_val : BitVec 64) : BitVec 64 :=
-  BitVec.extractLsb' 0 64
-    (BitVec.ofInt 65
-      (if ((2^63)-1) < if rs2_val.toInt = 0 then -1 else rs1_val.toInt.tdiv rs2_val.toInt then
-         -(2^63)
-      else if rs2_val.toInt = 0 then -1 else rs1_val.toInt.tdiv rs2_val.toInt))
-
-def DIV_pure64_signed_bv (rs2_val : BitVec 64) (rs1_val : BitVec 64) : BitVec 64 :=
-  if rs2_val = 0#64 then
-    -1#64
-  else
-    rs1_val.sdiv rs2_val
-
-theorem DIV_pure64_signed_eq_DIV_pure64_signed_bv (rs2_val : BitVec 64) (rs1_val : BitVec 64)  :
-  DIV_pure64_signed (rs2_val) (rs1_val ) = DIV_pure64_signed_bv (rs2_val) (rs1_val ) := by
-    unfold DIV_pure64_signed DIV_pure64_signed_bv
-    rw [extractLsb'_ofInt_eq_ofInt (h:= by simp)]
-    by_cases h1 : rs2_val = 0#64
-    case pos => simp [h1]
-    case neg =>
-      have h' : rs2_val.toInt ≠ 0 := by
-        have h1 := (BitVec.toInt_ne).mpr h1
-        exact h1
-      apply BitVec.eq_of_toInt_eq
-      simp only [Int.reduceSub, h', ↓reduceIte, Int.reduceNeg, BitVec.toInt_ofInt, h1]
-      simp only [Int.reducePow, Int.reduceSub, Int.reduceNeg, Nat.reducePow, BitVec.toInt_sdiv]
-      by_cases h : rs1_val = .intMin _ ∧ rs2_val = -1#64
-      case pos =>
-          obtain ⟨rfl, rfl⟩ := h
-          simp only [BitVec.toInt_intMin, Nat.add_one_sub_one, Nat.reducePow, Nat.reduceMod,
-            Nat.cast_ofNat, Int.reduceNeg, BitVec.reduceNeg, BitVec.reduceToInt, Int.tdiv_neg,
-            Int.tdiv_one, neg_neg, Int.reduceLT, ↓reduceIte, Int.reduceBmod]
-      case neg =>
-          have := BitVec.toInt_sdiv_of_ne_or_ne rs1_val rs2_val <| by
-              rw [← Decidable.not_and_iff_not_or_not]
-              exact h
-          rw[← this]
-          split
-          case isTrue iT =>
-            have intMax : (BitVec.intMax 64).toInt =  9223372036854775807 := by native_decide
-            have h3 : (rs1_val.sdiv rs2_val).toInt ≤2 ^ 63  - 1 := by
-                apply  BitVec.toInt_le
-            simp only [Int.reducePow, Int.reduceSub] at h3
-            exact (not_le_of_lt iT h3).elim
-          case isFalse iF =>
-          rfl
-
-def DIV_pure64_unsigned (rs2_val : BitVec 64) (rs1_val : BitVec 64) : BitVec 64 :=
-  BitVec.extractLsb' 0 64 (BitVec.ofInt 65 (if ((rs2_val.toNat):Int) = 0 then -1 else (rs1_val.toNat : Int).tdiv (rs2_val.toNat: Int)))
-
-def DIV_pure64_unsigned_bv (rs2_val : BitVec 64) (rs1_val : BitVec 64) : BitVec 64 :=
-  if rs2_val = 0#64 then  (-1)  else rs1_val.udiv rs2_val
-
-theorem  DIV_pure64_unsigned_eq_DIV_pure64_unsigned_bv (rs2_val : BitVec 64) (rs1_val : BitVec 64) :
-      DIV_pure64_unsigned (rs2_val ) (rs1_val)  = DIV_pure64_unsigned_bv (rs2_val ) (rs1_val) := by
-  unfold DIV_pure64_unsigned DIV_pure64_unsigned_bv
-  split
-  case isTrue ht =>
-      simp only [Int.reduceNeg, BitVec.reduceOfInt, extractLsb'_eq_setWidth, Nat.reduceLeDiff,
-        BitVec.setWidth_ofNat_of_le, BitVec.reduceOfNat, BitVec.ofNat_eq_ofNat, BitVec.reduceNeg,
-        BitVec.udiv_eq]
-      simp only [Int.natCast_eq_zero] at ht
-      have h3 :=  BitVec.eq_of_toNat_eq (x :=  rs2_val) (y:= 0) ht
-      simp only [h3, BitVec.ofNat_eq_ofNat, ↓reduceIte]
-  case isFalse hf =>
-      simp only [extractLsb'_eq_setWidth, BitVec.ofNat_eq_ofNat, BitVec.reduceNeg]
-      split
-      case isTrue htt =>
-          simp at hf
-          bv_omega
-      · rw [BitVec.setWidth_eq_extractLsb' (by simp)]
-        rw [extractLsb'_ofInt_eq_ofInt (h:= by simp)]
-        apply BitVec.eq_of_toInt_eq
-        simp only [BitVec.toInt_ofInt]
-        have aa := BitVec.isLt (rs1_val.udiv rs2_val)
-        rw [BitVec.udiv.eq_1 ]
-        rw[← Int.ofNat_tdiv]
-        rw [BitVec.toInt_eq_toNat_bmod]
-        simp only [Int.natCast_ediv, Nat.reducePow, BitVec.toNat_ofNatLT]
-
-def ITYPE_pure64_RISCV_ADDI (imm : BitVec 12) (rs1_val : BitVec 64) : BitVec 64 :=
-    let immext : BitVec 64 := (BitVec.signExtend 64 imm) ;
-    BitVec.add rs1_val immext
-
-def ITYPE_pure64_RISCV_SLTI (imm : BitVec 12) (rs1_val : BitVec 64) : BitVec 64 :=
-       let immext : BitVec 64 := (BitVec.signExtend 64 imm);
-       let b := BitVec.slt rs1_val immext;
-       BitVec.zeroExtend 64 (BitVec.ofBool b)
-
-def ITYPE_pure64_RISCV_SLTIU (imm : BitVec 12) (rs1_val : BitVec 64) : BitVec 64 :=
-       let immext : BitVec 64 := (BitVec.signExtend 64 imm);
-       let b := BitVec.ult rs1_val immext;
-       BitVec.setWidth 64 (BitVec.ofBool b)
-
-def  ITYPE_pure64_RISCV_ANDI (imm : BitVec 12) (rs1_val : BitVec 64) : BitVec 64 :=
-    let immext : BitVec 64 := (BitVec.signExtend 64 imm);
-      BitVec.and rs1_val immext
-
-def ITYPE_pure64_RISCV_ORI (imm : BitVec 12) (rs1_val : BitVec 64) : BitVec 64 :=
-      let immext : BitVec 64 := (BitVec.signExtend 64 imm) ;
-      BitVec.or rs1_val immext
-
-def  ITYPE_pure64_RISCV_XORI (imm : BitVec 12) (rs1_val : BitVec 64) : BitVec 64 :=
-      let immext : BitVec 64 := (BitVec.signExtend 64 imm) ;
-      BitVec.xor rs1_val immext
-
-def ZICOND_RTYPE_pure64_RISCV_CZERO_EQZ (rs2_val : BitVec 64) (rs1_val : BitVec 64) :=
-      (if rs2_val = BitVec.zero 64 then BitVec.zero 64 else rs1_val)
-
-def ZICOND_RTYPE_pure64_RISCV_RISCV_CZERO_NEZ (rs2_val : BitVec 64) (rs1_val : BitVec 64) :=
-   (if rs2_val = BitVec.zero 64 then rs1_val else BitVec.zero 64)
-
-def ZBS_RTYPE_pure64_RISCV_BCLR (rs2_val : BitVec 64) (rs1_val : BitVec 64) :=
-  BitVec.and rs1_val (BitVec.not (BitVec.shiftLeft (BitVec.zeroExtend 64 1#1) (BitVec.extractLsb  5 0 rs2_val).toNat))
-
-def ZBS_RTYPE_pure64_RISCV_BCLR_bv (rs2_val : BitVec 64) (rs1_val : BitVec 64) :=
-  BitVec.and rs1_val (BitVec.not ((BitVec.zeroExtend 64 1#1) <<< (BitVec.extractLsb  5 0 rs2_val)))
-
-theorem ZBS_RTYPE_pure64_RISCV_BCLR_eq_ZBS_RTYPE_pure64_RISCV_BCLR_bv (rs2_val : BitVec 64) (rs1_val : BitVec 64) :
-  ZBS_RTYPE_pure64_RISCV_BCLR (rs2_val) (rs1_val) =  ZBS_RTYPE_pure64_RISCV_BCLR_bv (rs2_val) (rs1_val) :=
-    by
-    unfold ZBS_RTYPE_pure64_RISCV_BCLR ZBS_RTYPE_pure64_RISCV_BCLR_bv
-    bv_normalize
-
-def ZBB_EXTOP_pure64_RISCV_SEXTB (rs1_val : BitVec 64) :=
-  BitVec.signExtend 64 (BitVec.extractLsb 7 0 rs1_val)
-
-def ZBB_EXTOP_pure64_RISCV_SEXTH  (rs1_val : BitVec 64) :=
-  BitVec.signExtend 64 (BitVec.extractLsb 15 0 rs1_val)
-
-def ZBB_EXTOP_pure64_RISCV_ZEXTH  (rs1_val : BitVec 64) :=
-  BitVec.zeroExtend 64 (BitVec.extractLsb 15 0 rs1_val)
-
-def ZBS_RTYPE_pure64_RISCV_BEXT (rs2_val : BitVec 64) (rs1_val : BitVec 64)  :=
-  BitVec.setWidth 64
-    (match
-      BitVec.and rs1_val (BitVec.shiftLeft (BitVec.setWidth 64 1#1) (BitVec.extractLsb 5 0 rs2_val).toNat) !=
-        0#64 with
-    | true => 1#1
-    | false => 0#1)
-
-def ZBS_RTYPE_pure64_RISCV_BEXT_bv (rs2_val : BitVec 64) (rs1_val : BitVec 64)  :=
-  BitVec.setWidth 64
-    (match
-      BitVec.and rs1_val ( (BitVec.setWidth 64 1#1) <<< (BitVec.extractLsb 5 0 rs2_val)) !=
-        0#64 with
-    | true => 1#1
-    | false => 0#1)
-
-theorem ZBS_RTYPE_pure64_RISCV_BEXT_eq_ZBS_RTYPE_pure64_RISCV_BEXT_bv (rs2_val : BitVec 64) (rs1_val : BitVec 64) :
-  ZBS_RTYPE_pure64_RISCV_BEXT (rs2_val) (rs1_val) = ZBS_RTYPE_pure64_RISCV_BEXT_bv (rs2_val) (rs1_val) :=
-    by
-    unfold ZBS_RTYPE_pure64_RISCV_BEXT  ZBS_RTYPE_pure64_RISCV_BEXT_bv
-    simp
-
- def ZBS_RTYPE_pure64_BINV (rs2_val : BitVec 64) (rs1_val : BitVec 64) :=
-  BitVec.xor rs1_val  (BitVec.shiftLeft (BitVec.zeroExtend 64 1#1) (BitVec.extractLsb 5 0 rs2_val).toNat)
-
- def ZBS_RTYPE_pure64_BINV_bv (rs2_val : BitVec 64) (rs1_val : BitVec 64) :=
-  BitVec.xor rs1_val  ((BitVec.zeroExtend 64 1#1) <<< (BitVec.extractLsb 5 0 rs2_val))
-
-theorem ZBS_RTYPE_pure64_BINV_eq_ZBS_RTYPE_pure64_BINV_bv  (rs2_val : BitVec 64) (rs1_val : BitVec 64) :
-  ZBS_RTYPE_pure64_BINV (rs2_val) (rs1_val)  = ZBS_RTYPE_pure64_BINV_bv rs2_val rs1_val :=
-  by
-  unfold ZBS_RTYPE_pure64_BINV ZBS_RTYPE_pure64_BINV_bv
-  bv_decide
-
-def ZBS_RTYPE_pure64_RISCV_BSET (rs2_val : BitVec 64) (rs1_val : BitVec 64) :=
-  BitVec.or rs1_val (BitVec.shiftLeft (BitVec.zeroExtend 64 1#1) (BitVec.extractLsb 5 0 rs2_val).toNat)
-
-def ZBS_RTYPE_pure64_RISCV_BSET_bv (rs2_val : BitVec 64) (rs1_val : BitVec 64) :=
-  BitVec.or rs1_val ((BitVec.zeroExtend 64 1#1) <<< (BitVec.extractLsb 5 0 rs2_val))
-
-theorem ZBS_RTYPE_pure64_RISCV_BSET_eq_ZBS_RTYPE_pure64_RISCV_BSET_bv (rs2_val : BitVec 64) (rs1_val : BitVec 64) :
-  ZBS_RTYPE_pure64_RISCV_BSET (rs2_val) (rs1_val) = ZBS_RTYPE_pure64_RISCV_BSET_bv (rs2_val) (rs1_val) :=
-   by
-   unfold ZBS_RTYPE_pure64_RISCV_BSET ZBS_RTYPE_pure64_RISCV_BSET_bv
-   simp
-
-def ZBS_IOP_pure64_RISCV_BCLRI (shamt : BitVec 6) (rs1_val : BitVec 64) :=
-  BitVec.and rs1_val (BitVec.not (BitVec.shiftLeft (BitVec.setWidth 64 1#1) (shamt.toNat)))
-
-def ZBS_IOP_pure64_RISCV_BCLRI_bv (shamt : BitVec 6) (rs1_val : BitVec 64) :=
-  BitVec.and rs1_val (BitVec.not ( (BitVec.setWidth 64 1#1) <<< shamt))
-
-theorem ZBS_IOP_pure64_RISCV_BCLRI_eq_ZBS_IOP_pure64_RISCV_BCLRI_bv (shamt : BitVec 6) (rs1_val : BitVec 64) :
-   ZBS_IOP_pure64_RISCV_BCLRI (shamt) (rs1_val ) = ZBS_IOP_pure64_RISCV_BCLRI_bv (shamt) (rs1_val) :=
-    by
-    unfold  ZBS_IOP_pure64_RISCV_BCLRI ZBS_IOP_pure64_RISCV_BCLRI_bv
-    simp
-
-def ZBS_IOP_pure64_RISCV_BEXTI (shamt : BitVec 6) (rs1_val : BitVec 64) :=
-  BitVec.setWidth 64
-      (match (BitVec.and (rs1_val) (BitVec.shiftLeft (BitVec.setWidth 64 1#1) shamt.toNat)) != 0#64 with
-      | true => 1#1
-      | false => 0#1)
-
-def ZBS_IOP_pure64_RISCV_BEXTI_bv (shamt : BitVec 6) (rs1_val : BitVec 64) :=
-  BitVec.setWidth 64
-      (match (BitVec.and (rs1_val) ( (BitVec.setWidth 64 1#1) <<< shamt)) != 0#64 with
-      | true => 1#1
-      | false => 0#1)
-
-theorem  ZBS_IOP_pure64_RISCV_BEXTI_eq_ZBS_IOP_pure64_RISCV_BEXTI_bv (shamt : BitVec 6) (rs1_val : BitVec 64) :
-  ZBS_IOP_pure64_RISCV_BEXTI (shamt) (rs1_val ) = ZBS_IOP_pure64_RISCV_BEXTI_bv (shamt ) (rs1_val ) :=
-  by
-  unfold ZBS_IOP_pure64_RISCV_BEXTI  ZBS_IOP_pure64_RISCV_BEXTI_bv
-  simp
-
-def ZBS_IOP_pure64_RISCV_BINVI (shamt : BitVec 6) (rs1_val : BitVec 64) :=
-  BitVec.xor rs1_val  (BitVec.shiftLeft (BitVec.zeroExtend 64 1#1) shamt.toNat)
-
-def ZBS_IOP_pure64_RISCV_BINVI_bv (shamt : BitVec 6) (rs1_val : BitVec 64) :=
-  BitVec.xor rs1_val  ( (BitVec.zeroExtend 64 1#1) <<< shamt)
-
-theorem ZBS_IOP_pure64_RISCV_BINVI_eq_ZBS_IOP_pure64_RISCV_BINVI_bv (shamt : BitVec 6) (rs1_val : BitVec 64) :
-  ZBS_IOP_pure64_RISCV_BINVI (shamt) (rs1_val) = ZBS_IOP_pure64_RISCV_BINVI_bv (shamt ) (rs1_val) :=
-   by
-   unfold ZBS_IOP_pure64_RISCV_BINVI ZBS_IOP_pure64_RISCV_BINVI_bv
-   rfl
-
-def ZBS_IOP_pure64_RISCV_BSETI (shamt : BitVec 6) (rs1_val : BitVec 64) :=
-  BitVec.or rs1_val (BitVec.shiftLeft (BitVec.zeroExtend 64 1#1) shamt.toNat)
-
-def ZBS_IOP_pure64_RISCV_BSETI_bv (shamt : BitVec 6) (rs1_val : BitVec 64) :=
-  BitVec.or rs1_val ((BitVec.zeroExtend 64 1#1) <<< shamt)
-
-theorem ZBS_IOP_pure64_RISCV_BSETI_eq_ZBS_IOP_pure64_RISCV_BSETI_bv (shamt : BitVec 6) (rs1_val : BitVec 64) :
-  ZBS_IOP_pure64_RISCV_BSETI (shamt) (rs1_val) =   ZBS_IOP_pure64_RISCV_BSETI_bv (shamt) (rs1_val) :=
-    by
-    unfold ZBS_IOP_pure64_RISCV_BSETI  ZBS_IOP_pure64_RISCV_BSETI_bv
-    simp
-
--- won't ever transform this
-def ZBB_RTYPEW_pure64_RISCV_RORW (rs2_val : BitVec 64) (rs1_val : BitVec 64) :=
-  BitVec.signExtend (64)
-      (BitVec.or (BitVec.ushiftRight (BitVec.setWidth 32 rs1_val) (rs2_val.toNat % 32))
-        (BitVec.shiftLeft (BitVec.setWidth 32 rs1_val)
-          ((2 ^ 5 - rs2_val.toNat % 32 +
-              32 % 2 ^ (5 + 1)) %
-            2 ^ 5)))
-
-def ZBB_RTYPEW_pure64_RISCV_ROLW (rs2_val : BitVec 64) (rs1_val : BitVec 64) :=
-BitVec.signExtend 64
-    (BitVec.or (BitVec.shiftLeft (BitVec.setWidth 32 rs1_val) (BitVec.extractLsb 4 0 rs2_val).toNat)
-      (BitVec.ushiftRight (BitVec.setWidth 32 rs1_val) (
-        ((BitVec.sub ((BitVec.extractLsb' 0 (5)
-            (BitVec.ofInt (6)
-              (32))))
-          (BitVec.extractLsb 4 0 rs2_val)))).toNat))
-
- def ZBB_RTYPE_pure64_RISCV_ROL (rs2_val : BitVec 64) (rs1_val : BitVec 64) :=
-  BitVec.or (BitVec.shiftLeft  rs1_val (BitVec.extractLsb 5 0 rs2_val).toNat)
-    (BitVec.ushiftRight rs1_val  (BitVec.extractLsb' 0 6 (BitVec.ofInt (7) (64)) - BitVec.extractLsb 5 0 rs2_val).toNat)
-
- def ZBB_RTYPE_pure64_RISCV_ROL_bv  (rs2_val : BitVec 64) (rs1_val : BitVec 64) :=
-  BitVec.or (BitVec.shiftLeft  rs1_val (BitVec.extractLsb 5 0 rs2_val).toNat)
-    (rs1_val >>> (BitVec.extractLsb' 0 6 (64#7) - BitVec.extractLsb 5 0 rs2_val))
-
-theorem ZBB_RTYPE_pure64_RISCV_ROL_eq_ZBB_RTYPE_pure64_RISCV_ROL_bv  (rs2_val : BitVec 64) (rs1_val : BitVec 64)  :
-  ZBB_RTYPE_pure64_RISCV_ROL  (rs2_val ) (rs1_val ) =  ZBB_RTYPE_pure64_RISCV_ROL_bv  (rs2_val) (rs1_val) :=
-    by
-    unfold ZBB_RTYPE_pure64_RISCV_ROL ZBB_RTYPE_pure64_RISCV_ROL_bv
-    simp
-
- def ZBB_RTYPE_pure64_RISCV_ROR (rs2_val : BitVec 64) (rs1_val : BitVec 64) :=
-      BitVec.or (BitVec.ushiftRight rs1_val (BitVec.extractLsb 5 0 rs2_val).toNat)
-    (BitVec.shiftLeft rs1_val ((BitVec.extractLsb' 0 6 (BitVec.ofInt (7) (64)) - BitVec.extractLsb 5 0 rs2_val)).toNat)
-
- def ZBB_RTYPE_pure64_RISCV_ROR_bv (rs2_val : BitVec 64) (rs1_val : BitVec 64) :=
-      BitVec.or ( rs1_val >>> (BitVec.extractLsb 5 0 rs2_val))
-    ( rs1_val  <<<  ((BitVec.extractLsb' 0 6 (BitVec.ofInt (7) (64)) - BitVec.extractLsb 5 0 rs2_val)))
-
-theorem ZBB_RTYPE_pure64_RISCV_ROR_eq_ZBB_RTYPE_pure64_RISCV_ROR_bv (rs2_val : BitVec 64) (rs1_val : BitVec 64) :
-  ZBB_RTYPE_pure64_RISCV_ROR (rs2_val) (rs1_val) = ZBB_RTYPE_pure64_RISCV_ROR_bv (rs2_val) (rs1_val) :=
-    by
-    unfold ZBB_RTYPE_pure64_RISCV_ROR  ZBB_RTYPE_pure64_RISCV_ROR_bv
-    simp
-
- def ZBA_RTYPEUW_pure64_RISCV_ADDUW (rs2_val : BitVec 64) (rs1_val : BitVec 64) :=
-      BitVec.zeroExtend 64 (BitVec.extractLsb 31 0 rs1_val) <<< 0#2 + rs2_val
-
-def  ZBA_RTYPEUW_pure64_RISCV_SH1ADDUW (rs2_val : BitVec 64) (rs1_val : BitVec 64) :=
-    BitVec.add (BitVec.zeroExtend (64) (BitVec.extractLsb 31 0 rs1_val) <<< 1#2)  (rs2_val)
-
-def ZBA_RTYPEUW_pure64_RISCV_SH2ADDUW (rs2_val : BitVec 64) (rs1_val : BitVec 64) :=
-      BitVec.add (BitVec.zeroExtend (64) (BitVec.extractLsb 31 0 rs1_val) <<< 2#2) rs2_val
-
-def  ZBA_RTYPEUW_pure64_RISCV_SH3ADDUW (rs2_val : BitVec 64) (rs1_val : BitVec 64) :=
-      BitVec.add (BitVec.zeroExtend (64) (BitVec.extractLsb 31 0 rs1_val) <<< 3#2)  rs2_val
-
-def ZBA_RTYPE_pure64_RISCV_SH1ADD (rs2_val : BitVec 64) (rs1_val : BitVec 64) :=
-    BitVec.add (rs1_val <<< 1#2) rs2_val
-
-def ZBA_RTYPE_pure64_RISCV_SH2ADD (rs2_val : BitVec 64) (rs1_val : BitVec 64) :=
-    BitVec.add (rs1_val <<< 2#2) rs2_val
-
-def ZBA_RTYPE_pure64_RISCV_SH3ADD(rs2_val : BitVec 64) (rs1_val : BitVec 64) :=
-    BitVec.add (rs1_val <<< 3#2) rs2_val
-
-/-
-to complete in the future:
-def ZBB_RYTPE_pure64_RISCV_ + rytpe from sail side is missing.
-|pack
-|packh
-slli.uw
- -/
 end pure_semantics
